%%%%%%%%%%%%%%%%%%%%%%%%%%%%%%%%%%%%%%%%%
% Lachaise Assignment
% LaTeX Template
% Version 1.0 (26/6/2018)
%
% This template originates from:
% http://www.LaTeXTemplates.com
%
% Authors:
% Marion Lachaise & François Févotte
% Vel (vel@LaTeXTemplates.com)
%
% License:
% CC BY-NC-SA 3.0 (http://creativecommons.org/licenses/by-nc-sa/3.0/)
% 
%%%%%%%%%%%%%%%%%%%%%%%%%%%%%%%%%%%%%%%%%

%----------------------------------------------------------------------------------------
%	PACKAGES AND OTHER DOCUMENT CONFIGURATIONS
%----------------------------------------------------------------------------------------

\documentclass{article}

\input{structure.tex} % Include the file specifying the document structure and custom commands

%----------------------------------------------------------------------------------------
%	ASSIGNMENT INFORMATION
%----------------------------------------------------------------------------------------

\title{Fourier Analysis Stein: Chapter 8. Problems.} % Title of the assignment

\author{Kelvin Hong\\ \texttt{kh.boon2@gmail.com}} % Author name and email address

\date{Xiamen University Malaysia, Asia Pacific University Malaysia --- \today} % University, school and/or department name(s) and a date

%----------------------------------------------------------------------------------------

\begin{document}

\maketitle % Print the title

\section{Problems}

\begin{enumerate}
    \item Prove that there are infinitely many primes by observing that if there were only finitely many, $p_1, \dots, p_N$, then
    $$\prod_{j=1}^N \dfrac1{1-1/p_j} \geq \sum_{n=1}^\infty \dfrac1n.$$

    \begin{solution}
        Assumes there are only finitely many primes $p_1, \dots, p_N$.
        Given a positive integer $M$, each positive integer $n\leq M$ can be expressed as a product of primes $p_1^{k_1} \cdots p_N^{k_N}$ for some
        integers $k_1, \dots, k_N$.
        We let $K_1, \dots, K_N$ be the maximum values of $k_1, \dots, k_N$ across all $n\leq M$.
        Thus, we have 
        \begin{align*}
            \prod_{j=1}^N \dfrac1{1-1/p_j} &\geq \prod_{j=1}^N \left(\sum_{k=0}^{K_j} \dfrac1{p_j^k}\right) \geq \sum_{n=1}^M \dfrac1n.
        \end{align*}
        Taking the limit as $M\to\infty$, we see that the RHS diverges, which is a contradiction to our assumption.
    \end{solution}

    \item In the text we showed that there are infinitely many primes of the form $4k+3$ by a modification of Euclid's original argument.
    Adapt this technique to prove the similar result for primes of the form $3k+2$, and for those of the form $6k+5$.

    \begin{solution}
        Assume there are only finitely many primes of the form $3k+2$, and let $p_1, \dots, p_N$ be all of them in increasing order and $p_1=5$.
        Consider the number $n=3p_1\cdots p_N+2$. This is a number of the form $3k+2$ and $n>p_N$, so it must be composite by our assumption.
        Since it is not divisible by $3$, it must have prime factors of the form $3k+1$ and $3k+2$.
        If it only has prime factors of the form $3k+1$, the product of these primes would be still of the form $3k+1$, so it
        will at least has a prime factor of the form $3k+2$. But this is a contradiction since $n$ is not divisible by any of the primes $p_1, \dots, p_N$.

        For another solution, we assume there are only finitely many primes of the form $6k+5$, $q_1, \dots, q_M$, in increasing order,
        where $q_1=11$.
        We can let $m=6q_1\cdots q_M+5$, we can argue similarly by noting that if $m$ is composite, it must have prime factors of the form
        $6k+1$ and $6k+5$, and also it must have at least one prime factor of the form $6k+5$, which create a contradiction.
    \end{solution}

    \item Prove that if $p$ and $q$ are relatively prime, then $\mathbb Z^* (p) \times \mathbb Z^* (q)$ is isomorphic to $\mathbb Z^* (pq)$.
    
    \begin{solution}
        Let $\phi: \mathbb Z^* (p) \times \mathbb Z^* (q) \to \mathbb Z^* (pq)$ be defined by $\phi(a,b) = aq+bp \mod pq$.
        Obviously both sets are groups, so we only need to show the mapping is one-to-one and surjective.

        To show $\phi$ is one-to-one, suppose $\phi(a,b) = \phi(c,d)$, then $aq+bp \equiv cq+dp \mod pq$. There is an integer $k$ such that
        $(a-c)q+(b-d)p = kpq.$ Rearrange to get $(a-c)q = p(kq-b+d)$. Since $p$ and $q$ are relatively prime, $p$ divides $a-c$, hence $a\equiv c\pmod p$.
        Similarly $b\equiv d\pmod q$.

        To show $\phi$ is surjective, we first let $x,y$ be integers such that $py+qx\equiv 1\pmod pq$ with $x\in\mathbb Z^*(p)$ and $y\in\mathbb Z^*(q)$.
        For any $z\in\mathbb Z^*(pq)$, we can write $z = z\cdot 1 = z(py+qx) = zpy+zqx$. We find that $\phi(zx, zy) = z$ just because $z$ is
        both relatively prime to $p$ and $q$. 
    \end{solution}

    \item (Skipped)
    \item If $n$ is a positive integer, show that
    $$n=\sum_{d|n}\varphi(d),$$
    where $\varphi$ is the Euler phi-function.

    \begin{solution}
        For any $1\leq d\leq n$, if $d$ is a divisor of $n$, then $\varphi(n/d)$ is the number of integers $1\leq k\leq n/d$ such that
        $\gcd(k, n/d)=1$. Let $m=kd$, then we have $\gcd(m, n)=d$. We see there are exactly $\varphi(n/d)$ integers $m$ satisfying
        $\gcd(m,n)=d$.

        Obviously for each $1\leq m\leq n$, $\gcd(m,n)$ is a divisor of $d$, so we actually have
        $$n=\sum_{d|n} \varphi(n/d) = \sum_{d|n}\varphi(d).$$
    \end{solution}

    \item (Skipped)
    \item Recall that for $\abs{z} < 1$, 
    $$\log_1\left(\dfrac1{1-z}\right) = \sum_{k\geq 1}\dfrac{z^k}k.$$
    We have seen that 
    $$e^{\log_1\left(\dfrac1{1-z}\right)} = \dfrac1{1-z}.$$
    \begin{enumerate}
        \item Show that if $w=1/(1-z)$, then $\abs z<1$ if and only if $\Re(w)>1/2$.

        \begin{solution}
            We rearrange to see $z=1-1/w$, so $\abs z<1$ iff $1-\frac1w-\frac1{\bar w}+\frac1{\abs w^2}<1$, we then have
            $$\dfrac1{\abs w^2} < \dfrac1 w+\dfrac1 {\bar w}  = \dfrac{w+\bar w}{\abs w^2} = \dfrac{2\Re(w)}{\abs w^2}.$$
            Since the above derivation are all equivalent, we have $\abs z<1$ iff $\Re(w)>1/2$.
        \end{solution}
        \item Show that if $\Re(w)>1/2$ and $w=\rho e^{i\varphi}$ with $\rho>0, \abs \varphi<\pi$, then
        $$\log_1 w = \log \rho + i\varphi.$$
        \begin{solution}
            We have $e^{\log_1w}=w$, so there is an integer $k$ such that $\log_1w = \log \rho + i(2\pi + \varphi)$.
            Now view $\log_1w$ as a function of $\varphi$, when $\varphi=0$ we have that $\log_1w$ is real, and is exactly $\log\rho$,
            since $k$ is an integer, it must be zero.
        \end{solution}
    \end{enumerate}

    \item Let $\zeta$ denote the zeta function defined for $s>1$. 
    \begin{enumerate}
        \item Compare $\zeta(s)$ with $\int_1^\infty x^{-s}dx$ to show that 
        $$\zeta(s) = \dfrac1{s-1} + O(1) \quad\text{ as }s\to 1^+.$$

        \begin{solution}
            For each integer $N\geq 2$ we let $\zeta_N(s) = \sum_{n=1}^N n^{-s}$, we have
            \begin{align*}
                \zeta_N(s)&\leq 1+\sum_{n=2}^N \int_{n-1}^n x^{-s}dx\\
                &=1+\int_1^N x^{-s}dx\\
                &= 1+\dfrac1{s-1} - \dfrac1{(s-1)N^{s-1}}\\
                &< 1+\dfrac1{s-1}.
            \end{align*}
            By letting $N\to\infty$, we see $\zeta(s) \leq \dfrac1{s-1} + 1$ for every $s>1$.
            Similarly, if we fixed $s>1$, we have
            $$\zeta_N(s) \geq \int_1^{N+1} x^{-s}dx = \dfrac1{s-1} - \dfrac{1}{(s-1)(N+1)^{s-1}} \implies \zeta(s) \geq \dfrac1{s-1}.$$
            Hence this also hold for every $s>1$. Note that we actually proved something stronger:
            $$\dfrac1{s-1} \leq \zeta(s) \leq \dfrac1{s-1} + 1.$$
        \end{solution}
        \item Prove as a consequence that 
        $$\sum_p \dfrac1{p^s} = \log\left(\dfrac1{s-1}\right) + O(1)\quad\text{ as } s\to 1^+.$$
        \begin{solution}
            Note that $\zeta(s) = \prod_p \dfrac1{1-p^{-s}}$, taking logarithm both sides give us
            \begin{align*}
                \log\zeta(s) &= -\sum_p \log\left(1-\dfrac1{p^s}\right) \\
                &= \sum_p \left(\dfrac1{p^s} + \sum_{k\geq 2} \dfrac1{k p^{ks}}\right)\\
            \end{align*}
            The second term can be bounded as below:
            $$0\leq \sum_{k\geq 2} \dfrac1{k p^{ks}} \leq \frac12 \sum_{k\geq 2} \dfrac1{p^{ks}} = \frac12 \cdot \dfrac{p^{-2s}}{1-p^{-s}}\leq p^{-2s}$$
            which gives us
            $$\log\zeta(s) = \sum_p \dfrac1{p^s} + \sum_p O\left(\dfrac1{p^{2s}}\right) = \sum_p \dfrac1{p^s} + O(1).$$
            When taking $s\to 1^+$, we have proved the result.
        \end{solution}
    \end{enumerate}
    \item Let $\chi_0$ denote that trivial Dirichlet character mod $q$, and $p_1, \dots, p_k$ the distinct prime divisors of $q$.
    Recall that $L(s, \chi_0)=(1-p_1^{-s})\cdots (1-p_k^{-s})\zeta(s)$, and show as a consequence
    $$L(s, \chi_0) = \dfrac{\varphi(q)}{q} \dfrac1{s-1} + O(1) \quad\text{ as } s \to 1^+.$$

    \begin{solution}
        We let $f(s) = (1-p_1^{-s})\cdots (1-p_k^{-s})$, then $f(1)=\varphi(q)/q$. Notice that $f$ is continuous at $s=1$ and has bounded
        derivative around $s=1$, which means
        $$\lim_{s\to 1+} \dfrac{f(s) - f(1)}{s-1}\quad\text{ is bounded.}$$
        By that and the previous exercise we have
        $$L(s, \chi_0) = \dfrac{f(s)}{s-1} + O(f(s))=\dfrac{\varphi(q)}q \dfrac{1}{s-1} + \dfrac{f(s)-f(1)}{s-1} + O(1)=
            \dfrac{\varphi(q)}q \dfrac{1}{s-1} + O(1)$$
        as $s\to 1^+$.
    \end{solution}
    \item Show that if $\ell$ is relatively prime to $q$, then
    $$\sum_{p\equiv \ell} \dfrac{1}{p^s} = \dfrac1{\varphi(q)}\log\left(\dfrac1{s-1}\right) + O(1) \quad\text{ as } s\to 1^+.$$
    This is a quantitative version of Dirichlet's theorem.

    \begin{solution}
        Using formula (4) in this chapter, we already know the second term on the RHS is $O(1)$, and since there are only finitely many primes as divisor of $q$, together
        with previous exercise it naturally gives us the result here.
    \end{solution}
    \item Use the characters for $\mathbb Z^*(3), \mathbb Z^*(4), \mathbb Z^*(5)$, and $\mathbb Z^*(6)$ to verify
    directly  that $L(1, \chi)\neq 0$ for all non-trivial Dirichlet characters modulo $q$ when
    $q=3,4,5$, and $6$.

    \begin{solution}
        In $\mathbb Z^*(3)$, the only non-trivial character satisfies $\chi(3k)=0, \chi(3k+1)=1, \chi(3k+2)=-1$, so 
        $$L(1, \chi) = \sum_{k=0}^\infty \left(\frac1{3k+1} - \frac1{3k+2}\right) = \sum_{k=0}^\infty \dfrac1{(3k+1)(3k+2)}.$$
        This is a positive sum and also $L(1, \chi) \neq 0$.
        The same argument can be applied to $\mathbb Z^*(4), \mathbb Z^*(6)$ as we can get $L(1, \chi) = \sum_{k=0}^\infty \dfrac2{(4k+1)(4k+3)}$
        and $\sum_{k=0}^\infty \dfrac4{(6k+1)(6k+5)}$ respectively.

        For $\mathbb Z^*(5)$, there are three non-trivial characters, solely depends on whether $\chi(5k+2)=-1, i, -i$.
        We can see that 
        $$\chi(5k+2)=-1 \implies L(1, \chi) = \sum_{k=0}^\infty \left(\dfrac1{(5k+1)(5k+2)} - \dfrac1{(5k+3)(5k+4)}\right) > 0;$$
        $$\chi(5k+2)=i \implies L(1, \chi) = \sum_{k=0}^\infty \dfrac3{(5k+1)(5k+4)} + i\sum_{k=0}^\infty \dfrac1{(5k+2)(5k+3)} \neq 0;$$
        $$\chi(5k+2)=-i \implies L(1, \chi) = \sum_{k=0}^\infty \dfrac3{(5k+1)(5k+4)} - i\sum_{k=0}^\infty \dfrac1{(5k+2)(5k+3)} \neq 0.$$
    \end{solution}
\end{enumerate}

\end{document}
